core/properties/distributivity/sampleMoore_distributivity.v
@@ -14,8 +14,8 @@
 
  
 
-Definition Moore_m1 : Model Metamodel_Instance :=
-    (Build_Model Metamodel_Instance
+Definition Moore_m1 : Model MooreMM :=
+    (Build_Model MooreMM
        (
         (TransitionElement (BuildTransition  "0")) :: 
         (TransitionElement (BuildTransition  "1")) :: nil
@@ -25,18 +25,18 @@ Definition Moore_m1 : Model Metamodel_Instance :=
        )
     ).
 
-Definition Moore_m2 : Model Metamodel_Instance :=
-       (Build_Model Metamodel_Instance
+Definition Moore_m2 : Model MooreMM :=
+       (Build_Model MooreMM
            (
                (StateElement (BuildState  "S0" "1")) :: 
                (StateElement (BuildState  "S1" "0")) ::  
                nil
            )
            (
-               (TransitionSourceLink (BuildTransitionSource (BuildTransition  "0") (BuildState  "S1" "0"))) ::
-               (TransitionTargetLink (BuildTransitionTarget (BuildTransition  "0") (BuildState  "S0" "1"))) ::
-               (TransitionSourceLink (BuildTransitionSource (BuildTransition  "1") (BuildState  "S0" "1"))) ::
-               (TransitionTargetLink (BuildTransitionTarget (BuildTransition  "1") (BuildState  "S1" "0"))) ::
+               (Transition_sourceLink (BuildTransitionSource (BuildTransition  "0") (BuildState  "S1" "0"))) ::
+               (Transition_targetLink (BuildTransitionTarget (BuildTransition  "0") (BuildState  "S0" "1"))) ::
+               (Transition_sourceLink (BuildTransitionSource (BuildTransition  "1") (BuildState  "S0" "1"))) ::
+               (Transition_targetLink (BuildTransitionTarget (BuildTransition  "1") (BuildState  "S1" "0"))) ::
                nil
            )
        ).
