core/properties/monotonicity/sampleMoore_monotonicity.v
@@ -14,8 +14,8 @@
 (* Moore models as counterexample to prove monotonicity of CoqTL *)
 
 
- Definition Moore_m1 : Model Metamodel_Instance :=
-     (Build_Model Metamodel_Instance
+ Definition Moore_m1 : Model MooreMM :=
+     (Build_Model MooreMM
         (
             (StateElement (BuildState  "S0" "1")) :: nil
         )
@@ -24,8 +24,8 @@
         )
      ).
  
-Definition Moore_m2 : Model Metamodel_Instance :=
-        (Build_Model Metamodel_Instance
+Definition Moore_m2 : Model MooreMM :=
+        (Build_Model MooreMM
             (
                 (TransitionElement (BuildTransition  "0")) :: 
                 (TransitionElement (BuildTransition  "1")) ::
@@ -34,10 +34,10 @@ Definition Moore_m2 : Model Metamodel_Instance :=
                 nil
             )
             (
-                (TransitionSourceLink (BuildTransitionSource (BuildTransition  "0") (BuildState  "S1" "0"))) ::
-		        (TransitionTargetLink (BuildTransitionTarget (BuildTransition  "0") (BuildState  "S0" "1"))) ::
-                (TransitionSourceLink (BuildTransitionSource (BuildTransition  "1") (BuildState  "S0" "1"))) ::
-		        (TransitionTargetLink (BuildTransitionTarget (BuildTransition  "1") (BuildState  "S1" "0"))) ::
+                (Transition_sourceLink (BuildTransitionSource (BuildTransition  "0") (BuildState  "S1" "0"))) ::
+		        (Transition_targetLink (BuildTransitionTarget (BuildTransition  "0") (BuildState  "S0" "1"))) ::
+                (Transition_sourceLink (BuildTransitionSource (BuildTransition  "1") (BuildState  "S0" "1"))) ::
+		        (Transition_targetLink (BuildTransitionTarget (BuildTransition  "1") (BuildState  "S1" "0"))) ::
                 nil
             )
         ).
