transformations/Moore2Mealy/MooreSemantics.v
@@ -5,51 +5,52 @@ Require Import Moore.
 Require Import core.Model.
 Require Import core.utils.Utils.
 
-Definition MooreMetamodel_toStates (m: list Element) : list State :=
-    optionList2List (map (fun s => get_E_Data State_K s) m).
+Definition MooreMetamodel_toStates (m: list Element) : list State_t :=
+    optionList2List (map (fun s => get_E_data State_K s) m).
 
-Definition MooreMetamodel_toTransitions (m: list Element) : list Transition :=
-    optionList2List (map (fun s => get_E_Data Transition_K s) m).
+Definition MooreMetamodel_toTransitions (m: list Element) : list Transition_t :=
+    optionList2List (map (fun s => get_E_data Transition_K s) m).
 
-Definition MooreMetamodel_allStates (m: MooreModel) : list State :=
+Definition MooreMetamodel_allStates (m: MooreModel) : list State_t :=
     MooreMetamodel_toStates m.(modelElements).
 
-Definition MooreMetamodel_allTransitions (m: MooreModel) : list Transition :=
+Definition MooreMetamodel_allTransitions (m: MooreModel) : list Transition_t :=
     MooreMetamodel_toTransitions m.(modelElements).
 
-Definition initialState (m: MooreModel) : option State :=
-    find (fun s => eqb "S0" s.(name)) (MooreMetamodel_allStates m).
+Definition initialState (m: MooreModel) : option State_t :=
+    find (fun s => eqb "S0" s.(State_name)) (MooreMetamodel_allStates m).
 
 
-Definition State_outTransitions (s: State) (m: MooreModel) : list Transition :=
+Definition State_outTransitions (s: State_t) (m: MooreModel) : list Transition_t :=
     filter (fun t => 
-        match (Transition_getSource t m) with
-        | Some s' => beq_State s s'
+        match (getTransition_source t m) with
+        | Some s' => State_t_beq s s'
         | None => false
         end)
         (MooreMetamodel_allTransitions m).
 
-Definition State_acceptTransition (s: State) (m: MooreModel) (i: string) : option Transition :=
-    find (fun t => eqb i t.(input)) (State_outTransitions s m).
+Definition State_acceptTransition (s: State_t) (m: MooreModel) (i: string) : option Transition_t :=
+    find (fun t => eqb i t.(Transition_input)) (State_outTransitions s m).
         
-Fixpoint executeFromState (m: MooreModel) (current: State) (remainingInput: list string) : list string :=
+Definition search m current i :=
+  let outTransition :=  State_acceptTransition current m i in
+  match outTransition with 
+    | Some t =>  getTransition_target t m
+    | None => None
+    end.
+
+Fixpoint executeFromState (m: MooreModel) (current: State_t) (remainingInput: list string) : list string :=
     match remainingInput with 
-    | i :: is => 
-        let outTransition :=  State_acceptTransition current m i in
-        let trgState := 
-            match outTransition with 
-            | Some t =>  Transition_getTarget t m
-            | None => None
-            end in
-        match trgState with
-        | Some s => s.(output) :: (executeFromState m s is)
+    | i :: is =>      
+        match search m current i with
+        | Some s => s.(State_output) :: (executeFromState m s is)
         | None => nil
         end
     | _ => nil 
     end.
 
 Definition Moore_execute (m: MooreModel) (input: list string) : list string :=
-    match (initialState m) with 
+    match initialState m with 
     | Some s => executeFromState m s input
     | None => nil
     end.
