transformations/Moore2Mealy/MooreWF.v
@@ -6,7 +6,7 @@ Definition unique_names (m:MooreModel) :=
   forall e1 e2,
   List.In (StateElement e1) m.(Model.modelElements) ->
   List.In (StateElement e2) m.(Model.modelElements) ->
-  e1.(name) = e2.(name) ->
+  e1.(State_name) = e2.(State_name) ->
   e1 = e2.
 
 
@@ -14,9 +14,9 @@ Lemma in_find :
   forall m n e,
     unique_names m ->
     List.In e (MooreMetamodel_allStates m) ->
-    e.(name) = n ->
+    e.(State_name) = n ->
     List.find
-           (fun s : State => (n =? s.(name))%string)
+           (fun s : State_t => (n =? s.(State_name))%string)
            (MooreMetamodel_allStates m) = 
          Some e.
 Proof.
@@ -31,7 +31,7 @@ Proof.
       apply ListUtils.optionList2List_In in IN2.
       apply List.in_map_iff in IN2.
       destruct IN2 as (a & T & IN2).
-      unfold get_E_Data in T.
+      unfold get_E_data in T.
       destruct a. 
       - PropUtils.inj T.
         exact IN2.
@@ -42,7 +42,7 @@ Proof.
       apply ListUtils.optionList2List_In in H0.
       apply List.in_map_iff in H0.
       destruct H0 as (a & T & H0).
-      unfold get_E_Data in T.
+      unfold get_E_data in T.
       destruct a. 
       - PropUtils.inj T.
         exact H0.
